WIP parse header with pn

src/QUIC.Spec.Base.fst
@@ -115,13 +115,23 @@ let has_payload_length
 : Tot bool
 = MLong? h && (not (MRetry? (MLong?.spec h)))
 
-let payload_length 
+let payload_and_pn_length 
   (h: header { has_payload_length h })
 : Tot U62.t
 = match MLong?.spec h with
   | MInitial _ pl _ _ -> pl
   | MZeroRTT pl _ _ -> pl
   | MHandshake pl _ _ -> pl
+
+module Secret = QUIC.Secret
+
+let payload_length 
+  (h: header { has_payload_length h })
+: Tot U62.secret
+= match MLong?.spec h with
+  | MInitial _ pl pnl _ -> Secret.to_u64 pl `Secret.sub` Secret.to_u64 pnl
+  | MZeroRTT pl pnl _ -> Secret.to_u64 pl `Secret.sub` Secret.to_u64 pnl
+  | MHandshake pl pnl _ -> Secret.to_u64 pl `Secret.sub` Secret.to_u64 pnl
 
 (* Correctness of a packet wrt. parsing parameters (cid_len, window) *)
 
@@ -130,3 +140,33 @@ module Secret = Lib.IntTypes
 let is_valid_header (h: header) (cid_len: nat) (last: nat) : Tot Type0 =
   (MShort? h ==> dcid_len h == cid_len) /\
   ((~ (is_retry h)) ==> PN.in_window (Secret.v (pn_length h) - 1) last (Secret.v (packet_number h)))
+
+module HD = Spec.Hash.Definitions
+module AEAD = Spec.Agile.AEAD
+
+let supported_hash = function
+  | HD.SHA1 | HD.SHA2_256 | HD.SHA2_384 | HD.SHA2_512 -> true
+  | _ -> false
+
+let supported_aead = function
+  | AEAD.AES128_GCM | AEAD.AES256_GCM | AEAD.CHACHA20_POLY1305 -> true
+  | _ -> false
+
+type ha = a:HD.hash_alg{supported_hash a}
+type ea = a:AEAD.alg{supported_aead a}
+
+// JP: this is Spec.Agile.Cipher.key_length
+let ae_keysize (a:ea) =
+  match a with
+  | AEAD.AES128_GCM -> 16
+  | _ -> 32
+
+let header_len_bound = 16500 // FIXME: this should be in line with the parser kind
+
+let max_cipher_length : n:nat {
+  forall a. {:pattern AEAD.max_length a \/ AEAD.tag_length a }
+    n <= AEAD.max_length a + AEAD.tag_length a
+} =
+  pow2 32 - header_len_bound
+
+type cbytes = b:bytes{let l = S.length b in 19 <= l /\ l < max_cipher_length}
