src/QUIC.Spec.Header.fst
@@ -2,6 +2,331 @@ module QUIC.Spec.Header
 open QUIC.Spec.Base
 
 module PN = QUIC.Spec.PacketNumber
+module Public = QUIC.Spec.Public
+module LP = LowParse.Spec.Combinators
+module Secret = QUIC.Secret
+module BF = LowParse.BitFields
+module U8 = FStar.UInt8
+
+let protected_bits_pn_length
+  (is_short: bool)
+  (pb: Public.bitfield (if is_short then 5 else 4))
+: Tot PN.packet_number_length_t
+= Secret.to_u32 #Secret.U8 (1uy `Secret.add` Secret.get_bitfield #Secret.U8 pb 0ul 2ul)
+
+let get_pn_length
+  (h: Public.header)
+: Tot PN.packet_number_length_t 
+= protected_bits_pn_length (Public.PShort? h) (Public.get_protected_bits h)
+
+let protected_bits_reserved
+  (is_short: bool)
+  (pb: Public.bitfield (if is_short then 5 else 4))
+: Tot (Public.bitfield 2)
+= if is_short
+  then BF.uint8.BF.get_bitfield pb 3 5
+  else BF.uint8.BF.get_bitfield pb 2 4
+
+let get_reserved_bits
+  (h: Public.header)
+: Tot (Public.bitfield 2)
+= protected_bits_reserved (Public.PShort? h) (Public.get_protected_bits h)
+
+let check_public_header
+  (cid_len: Public.short_dcid_len_t)
+  (h: Public.header' cid_len)
+: Tot bool
+= if Public.is_retry h
+  then true
+  else get_reserved_bits h = 0uy
+
+let checked_header
+  (cid_len: Public.short_dcid_len_t)
+= LP.parse_filter_refine (check_public_header cid_len)
+
+let packet_number_opt
+  (cid_len: Public.short_dcid_len_t)
+  (last: PN.last_packet_number_t)
+  (h: checked_header cid_len)
+: Tot Type0
+= if Public.is_retry h
+  then unit
+  else PN.packet_number_t' last (get_pn_length h)
+
+let parse_packet_number_opt_kind = LP.strong_parser_kind 0 4 None
+
+let parse_packet_number_opt
+  (cid_len: Public.short_dcid_len_t)
+  (last: PN.last_packet_number_t)
+  (h: checked_header cid_len)
+: Tot (LP.parser parse_packet_number_opt_kind (packet_number_opt cid_len last h))
+= if Public.is_retry h
+  then LP.weaken parse_packet_number_opt_kind LP.parse_empty
+  else LP.weaken parse_packet_number_opt_kind (PN.parse_packet_number last (get_pn_length h))
+
+let packet_number_prop
+  (last: PN.last_packet_number_t)
+  (h: header)
+: Tot bool
+= if not (is_retry h)
+  then PN.in_window (Secret.v (pn_length h) - 1) (Secret.v last) (Secret.v (packet_number h))
+  else true
+
+module U32 = FStar.UInt32
+
+let short_dcid_len_prop
+  (short_dcid_len: Public.short_dcid_len_t)
+  (h: header)
+: Tot bool
+= if MShort? h
+  then dcid_len h = U32.v short_dcid_len
+  else true
+
+unfold
+let parse_header_prop
+  (short_dcid_len: Public.short_dcid_len_t)
+  (last: PN.last_packet_number_t)
+  (m: header)
+: Tot bool
+= short_dcid_len_prop short_dcid_len m &&
+  packet_number_prop last m
+
+inline_for_extraction
+type header'
+  (short_dcid_len: Public.short_dcid_len_t)
+  (last: PN.last_packet_number_t)
+= LP.parse_filter_refine (parse_header_prop short_dcid_len last)
+
+module Cast = FStar.Int.Cast
+
+let protected_bits_key_phase
+  (x: Public.bitfield 5)
+: GTot bool
+= BF.uint8.BF.get_bitfield x 2 3 = 1uy
+
+let mk_short_protected_bits
+  (key_phase: bool)
+  (pnl: PN.packet_number_length_t)
+: GTot (Public.bitfield 5)
+= BF.set_bitfield_bound #8 0 5 0 2 (Secret.v pnl - 1);
+  BF.set_bitfield_bound #8 (BF.set_bitfield #8 0 0 2 (Secret.v pnl - 1)) 5 2 3 (if key_phase then 1 else 0);
+  BF.uint8.BF.set_bitfield (BF.uint8.BF.set_bitfield 0uy 0 2 (U8.uint_to_t (Secret.v pnl - 1))) 2 3 (if key_phase then 1uy else 0uy)
+
+let protected_bits_pn_length_prop
+  (is_short: bool)
+  (pb: Public.bitfield (if is_short then 5 else 4))
+: Lemma
+  (Secret.v (protected_bits_pn_length is_short pb) == U8.v (BF.uint8.BF.get_bitfield pb 0 2) + 1)
+  [SMTPat (protected_bits_pn_length is_short pb)]
+= ()
+
+let mk_short_protected_bits_correct
+  (key_phase: bool)
+  (pnl: PN.packet_number_length_t)
+: Lemma
+  (
+    let b = mk_short_protected_bits key_phase pnl in
+    protected_bits_pn_length true b == pnl /\
+    protected_bits_reserved true b == 0uy /\
+    protected_bits_key_phase b == key_phase /\
+    True
+  )
+= 
+  BF.get_bitfield_zero 8 3 5
+
+#push-options "--z3rlimit 16 --max_fuel 2"
+
+let mk_short_protected_bits_complete
+  (pb: Public.bitfield 5 { protected_bits_reserved true pb == 0uy } )
+: Lemma
+  (
+    mk_short_protected_bits (protected_bits_key_phase pb) (protected_bits_pn_length true pb) == pb
+  )
+= BF.get_bitfield_zero 8 3 5;
+  let pb' = mk_short_protected_bits (protected_bits_key_phase pb) (protected_bits_pn_length true pb) in
+  BF.get_bitfield_full #5 (U8.v pb');
+  BF.get_bitfield_full #5 (U8.v pb);
+  BF.get_bitfield_size 5 8 (U8.v pb) 0 5;
+  BF.get_bitfield_size 5 8 (U8.v pb') 0 5;
+  assert_norm (BF.get_bitfield_partition_prop #8 (U8.v pb) (U8.v pb') 0 5 [2; 3] <==> (
+    (BF.uint8.BF.v (BF.uint8.BF.get_bitfield pb 0 2) == BF.uint8.BF.v (BF.uint8.BF.get_bitfield pb' 0 2)) /\
+    (BF.uint8.BF.v (BF.uint8.BF.get_bitfield pb 2 3) == BF.uint8.BF.v (BF.uint8.BF.get_bitfield pb' 2 3)) /\
+    (BF.uint8.BF.v (BF.uint8.BF.get_bitfield pb 3 5) == BF.uint8.BF.v (BF.uint8.BF.get_bitfield pb' 3 5))
+  ));
+  BF.get_bitfield_partition #8 (U8.v pb) (U8.v pb') 0 5 [2; 3]
+
+#pop-options
+
+let mk_long_protected_bits
+  (pnl: PN.packet_number_length_t)
+: GTot (Public.bitfield 4)
+= BF.set_bitfield_bound #8 0 4 0 2 (Secret.v pnl - 1);
+  BF.uint8.BF.set_bitfield 0uy 0 2 (U8.uint_to_t (Secret.v pnl - 1))
+
+let mk_long_protected_bits_correct
+  (pnl: PN.packet_number_length_t)
+: Lemma
+  (
+    let b = mk_long_protected_bits pnl in
+    protected_bits_pn_length false b == pnl /\
+    protected_bits_reserved false b == 0uy
+  )
+=
+  BF.get_bitfield_zero 8 2 4
+
+let mk_long_protected_bits_complete
+  (pb: Public.bitfield 4 { protected_bits_reserved false pb == 0uy } )
+: Lemma
+  (
+    mk_long_protected_bits (protected_bits_pn_length false pb) == pb
+  )
+= BF.get_bitfield_zero 8 2 4;
+  let pb' = mk_long_protected_bits (protected_bits_pn_length false pb) in
+  BF.get_bitfield_full #4 (U8.v pb');
+  BF.get_bitfield_full #4 (U8.v pb);
+  BF.get_bitfield_size 4 8 (U8.v pb) 0 4;
+  BF.get_bitfield_size 4 8 (U8.v pb') 0 4;
+  assert (
+      (BF.uint8.BF.v (BF.uint8.BF.get_bitfield pb 0 2) == BF.uint8.BF.v (BF.uint8.BF.get_bitfield pb' 0 2)) /\
+    (BF.uint8.BF.v (BF.uint8.BF.get_bitfield pb 2 4) == BF.uint8.BF.v (BF.uint8.BF.get_bitfield pb' 2 4))
+  );
+  BF.get_bitfield_partition_2_gen #8 0 2 4 (U8.v pb) (U8.v pb')
+
+let synth_header
+  (short_dcid_len: Public.short_dcid_len_t)
+  (last: PN.last_packet_number_t)
+  (x: dtuple2 (checked_header short_dcid_len) (packet_number_opt short_dcid_len last))
+: GTot (header' short_dcid_len last)
+= let (| h, pn |) = x in
+  match h with
+  | Public.PShort protected_bits spin dcid ->
+    MShort spin (protected_bits_key_phase protected_bits) dcid (protected_bits_pn_length true protected_bits) pn
+  | Public.PLong protected_bits version dcid scid spec ->
+    let pnl = protected_bits_pn_length false protected_bits in
+    MLong version dcid scid
+      begin match spec with
+      | Public.PRetry odcid ->
+        MRetry protected_bits odcid
+      | Public.PInitial token payload_and_pn_length ->
+        MInitial token payload_and_pn_length pnl pn
+      | Public.PHandshake payload_and_pn_length ->
+        MHandshake payload_and_pn_length pnl pn
+      | Public.PZeroRTT payload_and_pn_length ->
+        MZeroRTT payload_and_pn_length pnl pn
+      end
+
+let synth_header_recip
+  (short_dcid_len: Public.short_dcid_len_t)
+  (last: PN.last_packet_number_t)
+  (x: header' short_dcid_len last)
+: GTot (dtuple2 (checked_header short_dcid_len) (packet_number_opt short_dcid_len last))
+= match x with
+  | MShort spin key_phase dcid pnl pn ->
+    mk_short_protected_bits_correct key_phase pnl;
+    (| Public.PShort (mk_short_protected_bits key_phase pnl) spin dcid, pn |)
+  | MLong version dcid scid spec ->
+    begin match spec with
+    | MRetry unused odcid ->
+      (| Public.PLong unused version dcid scid (Public.PRetry odcid), () |)
+    | MInitial token payload_and_pn_length pnl pn ->
+      mk_long_protected_bits_correct pnl;
+      (| Public.PLong (mk_long_protected_bits pnl) version dcid scid (Public.PInitial token payload_and_pn_length), pn |)
+    | MHandshake payload_and_pn_length pnl pn ->
+      mk_long_protected_bits_correct pnl;
+      (| Public.PLong (mk_long_protected_bits pnl) version dcid scid (Public.PHandshake payload_and_pn_length), pn |)
+    | MZeroRTT payload_and_pn_length pnl pn ->
+      mk_long_protected_bits_correct pnl;
+      (| Public.PLong (mk_long_protected_bits pnl) version dcid scid (Public.PZeroRTT payload_and_pn_length), pn |)
+    end
+
+let synth_header_injective
+  (short_dcid_len: Public.short_dcid_len_t)
+  (last: PN.last_packet_number_t)
+: Lemma
+  (LP.synth_injective #(dtuple2 (checked_header short_dcid_len) (packet_number_opt short_dcid_len last)) #(header' short_dcid_len last)  (synth_header short_dcid_len last))
+  [SMTPat (LP.synth_injective #(dtuple2 (checked_header short_dcid_len) (packet_number_opt short_dcid_len last)) #(header' short_dcid_len last) (synth_header short_dcid_len last))]
+= LP.synth_inverse_intro' (synth_header_recip short_dcid_len last) (synth_header short_dcid_len last) (fun (x: dtuple2 (checked_header short_dcid_len) (packet_number_opt short_dcid_len last)) ->
+    let (| h, pn |) = x in
+    match h with
+    | Public.PShort protected_bits spin dcid ->
+      mk_short_protected_bits_complete protected_bits
+    | Public.PLong protected_bits version dcid scid spec ->
+      begin match spec with
+      | Public.PRetry odcid -> ()
+      | _ -> mk_long_protected_bits_complete protected_bits
+      end
+  );
+  LP.synth_inverse_synth_injective (synth_header short_dcid_len last) (synth_header_recip short_dcid_len last)
+
+let synth_header_inverse
+  (short_dcid_len: Public.short_dcid_len_t)
+  (last: PN.last_packet_number_t)
+: Lemma
+  (LP.synth_inverse #(dtuple2 (checked_header short_dcid_len) (packet_number_opt short_dcid_len last)) #(header' short_dcid_len last) (synth_header short_dcid_len last) (synth_header_recip short_dcid_len last))
+  [SMTPat (LP.synth_inverse #(dtuple2 (checked_header short_dcid_len) (packet_number_opt short_dcid_len last)) #(header' short_dcid_len last) (synth_header short_dcid_len last) (synth_header_recip short_dcid_len last))]
+= LP.synth_inverse_intro' (synth_header short_dcid_len last) (synth_header_recip short_dcid_len last) (fun (x: header' short_dcid_len last) ->
+    match x with
+    | MShort spin key_phase dcid pnl pn ->
+      mk_short_protected_bits_correct key_phase pnl
+    | MLong version dcid scid spec ->
+      begin match spec with
+      | MRetry unused odcid -> ()
+      | MInitial token payload_and_pn_length pnl pn ->
+        mk_long_protected_bits_correct pnl
+      | MHandshake payload_and_pn_length pnl pn ->
+        mk_long_protected_bits_correct pnl
+      | MZeroRTT payload_and_pn_length pnl pn ->
+        mk_long_protected_bits_correct pnl
+      end
+  )
+
+let parse_header_kind
+  (short_dcid_len: Public.short_dcid_len_t)
+: Tot LP.parser_kind
+= LP.parse_filter_kind (Public.parse_header_kind' short_dcid_len) `LP.and_then_kind` parse_packet_number_opt_kind
+
+let parse_header
+  (short_dcid_len: Public.short_dcid_len_t)
+  (last: PN.last_packet_number_t)
+: Tot (LP.parser (parse_header_kind short_dcid_len) (header' short_dcid_len last))
+=
+  LP.parse_dtuple2
+    #_ #(checked_header short_dcid_len)
+    (LP.parse_filter (Public.parse_header short_dcid_len) (check_public_header short_dcid_len))
+    #_ #(packet_number_opt short_dcid_len last)
+    (parse_packet_number_opt short_dcid_len last)
+  `LP.parse_synth`
+    (synth_header short_dcid_len last)
+
+
+(*
+let parse_header_ifthenelse_payload
+  (has_pn: bool)
+: Tot Type0
+= if has_pn
+  then PN.packet_number_t
+  else unit
+
+let parse_header_ifthenelse_payload_parser
+  (last: PN.last_packet_number_t)
+  (has_pn: bool)
+: Tot (k: LP.parser_kind & LP.parser k (parse_header_ifthenelse_payload has_pn))
+= if has_pn
+  then (| _, PN.parse_packet_number last 
+
+
+let parse_header_param
+  (cid_len: Public.short_dcid_len_t)
+  (last: PN.last_packet_number_t)
+: Tot LP.parse_ifthenelse_param
+= {
+  LP.parse_ifthenelse_tag_kind = Public.parse_header_kind' cid_len;
+  LP.parse_ifthenelse_tag_t = Public.header' cid_len;
+  LP.parse_ifthenelse_tag_parser = Public.parse_header cid_len;
+  LP.parse_ifthenelse_tag_cond = public_header_has_pn cid_len;
+  LP.parse_ifthenelse_payload_t = 
+}
+
 
 (*
 open QUIC.Spec.PacketNumber
@@ -126,27 +451,6 @@ let short_dcid_len_prop
   (h: header)
 : GTot Type0
 = (MShort? h ==> dcid_len h == U32.v short_dcid_len)
-
-let packet_number_prop
-  (last: last_packet_number_t)
-  (h: header)
-: GTot Type0
-= ((~ (is_retry h)) ==> in_window (U32.v (pn_length h) - 1) (U64.v last) (U64.v (packet_number h)))
-
-unfold
-let parse_header_prop
-  (short_dcid_len: short_dcid_len_t)
-  (last: last_packet_number_t)
-  (m: header)
-: GTot Type0
-= short_dcid_len_prop short_dcid_len m /\
-  packet_number_prop last m
-
-inline_for_extraction
-type header'
-  (short_dcid_len: short_dcid_len_t)
-  (last: last_packet_number_t)
-= (m: header { parse_header_prop short_dcid_len last m })
 
 
 #push-options "--z3rlimit 16"
